coq-osiris/theories/program_logic/pure/expr_rules.v
@@ -417,23 +417,6 @@ Section match_rules.
       by apply Hζ.
   Qed.
 
-  Lemma pure_eval_trywith `{Encode A} η e bs (φ : A -> Prop) ζ ζ' :
-    pure (eval η e) φ ζ ->
-    (∀ ex, ζ ex -> pure (match_exn η ex bs) φ ζ') ->
-    pure (eval η (ETryWith e bs)) φ ζ'.
-  Proof.
-    intros Heval Htryw. simpl_eval.
-    eapply pure_wp_try, pure_wp_mono; eauto with pure.
-  Qed.
-
-  Lemma pure_eval_try_with_cons `{Encode A} η ex p e bs (φ : A -> Prop) ζ :
-    pattern η p ex (λ η', pure (eval η' e) φ ζ) (pure (match_exn η ex bs) φ ζ) ->
-    pure (match_exn η ex (Branch (CExc p) e :: bs)) φ ζ.
-  Proof.
-    intros Hpat. simpl_match_exn.
-    eapply pure_wp_try, pure_wp_mono; eauto.
-  Qed.
-
   (* Currently unused *)
 
   Lemma pure_match_cons_unary `{Encode A} η v p e bs (φ : A -> Prop) Ψ :
@@ -1525,4 +1508,3 @@ Proof.
     induction a; intros; destruct v0; inv H4; eauto.
     cbn. f_equiv. eapply IHa; eauto. }
 Qed.
-
